share/pulse/examples/AutoLem.fst
@@ -1,0 +1,21 @@
+module AutoLem
+
+open Pulse.Lib.Pervasives
+
+assume val p : int -> vprop
+assume val q : int -> vprop
+
+[@@guided_autolem]
+assume
+val pq : i:int -> stt_ghost unit emp_inames (p i) (fun _ -> q i)
+
+(*
+
+```pulse
+fn test ()
+  requires p 42
+  ensures q 42
+{
+  ();
+}
+```
