share/pulse/examples/AutoLem2.fst
@@ -1,0 +1,269 @@
+module AutoLem2
+
+open Pulse.Lib.Pervasives
+open FStar.Tactics.V2
+
+(* Shadow the one in the library so its own primitive
+automation does not apply.*)
+assume
+val pts_to (#a:Type) (r:ref a) (#f:perm) ([@@@equate_by_smt] n:a) 
+    : vprop
+
+// assume
+// val gather (#a:Type) (r:ref a) (#x0 #x1:erased a) (#p0 #p1:perm)
+//   : stt_ghost unit
+//       (pts_to r #p0 x0 ** pts_to r #p1 x1)
+//       (fun _ -> pts_to r #(sum_perm p0 p1) x0 ** pure (x0 == x1))
+
+// [@@guided_autolem]
+assume
+val share2 (#a:Type) (#f:perm) (r:ref a) (#v:erased a)
+  : stt_ghost unit
+      (pts_to r #f v)
+      (fun _ -> pts_to r #(half_perm f) v ** pts_to r #(half_perm f) v)
+
+[@@guided_autolem]
+assume
+val gather2 (#a:Type) (r:ref a) (#f:perm) (#x0 #x1:erased a)
+  : stt_ghost unit
+      (pts_to r #(half_perm f) x0 ** pts_to r #(half_perm f) x1)
+      (fun _ -> pts_to r #f x0 ** pure (x0 == x1))
+
+
+#set-options "--print_implicits --print_full_names"
+
+// ```pulse
+// fn test_share1 (r : ref int) (f:perm)
+//   requires pts_to r #f 1
+//   ensures pts_to r #(half_perm f) 1
+//        ** pts_to r #(half_perm f) 1
+// {
+//   ()
+// }
+// ```
+
+// assume
+// val share (#a:Type) (r:ref a) (#v:erased a) (#p:perm)
+//   : stt_ghost unit
+//       (pts_to r #p v)
+//       (fun _ ->
+//        pts_to r #(half_perm p) v **
+//        pts_to r #(half_perm p) v)
+
+```pulse
+fn test_gather1 (r : ref int) (f:perm)
+  requires pts_to r #one_half 1
+        ** pts_to r #one_half 1
+  ensures pts_to r #full_perm 1
+{
+  ();
+}
+```
+
+```pulse
+fn test_gather1_exists (r : ref int) (f:perm)
+  requires (exists* v. pts_to r #(half_perm f) v)
+        ** pts_to r #(half_perm f) 1
+  ensures pts_to r #f 1
+{
+  ()
+}
+```
+
+```pulse
+fn test_gather2_exists (r : ref int) (f:perm)
+  requires pts_to r #(half_perm f) 1
+        ** (exists* v. pts_to r #(half_perm f) v)
+  ensures pts_to r #f 1
+{
+  ()
+}
+```
+
+```pulse
+fn test_gather3_exists (r : ref int) (f:perm)
+  requires (exists* v. pts_to r #(half_perm f) v)
+        ** (exists* v. pts_to r #(half_perm f) v)
+  ensures (exists* v. pts_to r #f v)
+{
+  // FIXME: scoping
+  admit()
+}
+```
+
+```pulse
+fn test_gather_het1 (r : ref int) (v:int) (f:perm)
+  requires pts_to r #(half_perm f) 1
+        ** pts_to r #(half_perm f) v
+  ensures pts_to r #f 1
+{
+  ()
+}
+```
+
+```pulse
+fn test_gather_het2 (r : ref int) (v:int) (f:perm)
+  requires pts_to r #(half_perm f) 1
+        ** pts_to r #(half_perm f) v
+  ensures pts_to r #f v
+{
+  ();
+}
+```
+
+
+```pulse
+fn test_gather2 (r : ref int)
+  requires pts_to r #(half_perm full_perm) 1
+        ** pts_to r #(half_perm (half_perm full_perm)) 1
+        ** pts_to r #(half_perm (half_perm full_perm)) 1
+  ensures pts_to r 1
+{
+  assert (pts_to r #(half_perm full_perm) 1 ** pts_to r #(half_perm full_perm) 1);
+  ()
+}
+```
+
+```pulse
+fn test_share2 (r : ref int)
+  requires pts_to r 1
+  ensures  pts_to r #(half_perm full_perm) 1
+        ** pts_to r #(half_perm (half_perm full_perm)) 1
+        ** pts_to r #(half_perm (half_perm full_perm)) 1
+{
+  ()
+}
+```
+
+```pulse
+fn test_share2_0 (r : ref int)
+  requires pts_to r 1
+  ensures  pts_to r #(half_perm (half_perm full_perm)) 1
+        ** pts_to r #(half_perm (half_perm full_perm)) 1
+        ** pts_to r #(half_perm (half_perm full_perm)) 1
+        ** pts_to r #(half_perm (half_perm full_perm)) 1
+{
+  ()
+}
+```
+
+```pulse
+fn need_quarter (r : ref int) (f:perm)
+  requires pts_to r #(half_perm (half_perm f)) 1
+  ensures  pts_to r #(half_perm (half_perm f)) 1
+{
+  ()
+}
+```
+
+```pulse
+fn test_call_quarter (r: ref int)
+  requires pts_to r 1
+  ensures  pts_to r 1
+{
+  need_quarter r full_perm;
+  gather r;
+  gather r;
+}
+```
+
+
+```pulse
+fn test_gather3 (r : ref int) (s : ref int)
+  requires pts_to r #(half_perm full_perm) 1
+        ** pts_to r #(half_perm full_perm) 1
+        ** pts_to s 2
+  ensures pts_to r 1 ** pts_to s 2
+{
+  ()
+}
+```
+
+```pulse
+fn test_share3 (r : ref int) (s : ref int)
+  requires pts_to r 1 ** pts_to s 2
+  ensures  pts_to r #(half_perm full_perm) 1
+        ** pts_to r #(half_perm full_perm) 1
+        ** pts_to s 2
+{
+  ()
+}
+```
+
+```pulse
+fn test_gather4 (r : ref int) (s : ref int)
+  requires pts_to r #(half_perm full_perm) 1
+        ** pts_to r #(half_perm full_perm) 1
+        ** pts_to s #(half_perm full_perm) 2
+        ** pts_to s #(half_perm full_perm) 2
+  ensures pts_to r 1 ** pts_to s 2
+{
+  ()
+}
+```
+
+```pulse
+fn test_share4 (r : ref int) (s : ref int)
+  requires pts_to r 1 ** pts_to s 2
+  ensures  pts_to r #(half_perm full_perm) 1
+        ** pts_to r #(half_perm full_perm) 1
+        ** pts_to s #(half_perm full_perm) 2
+        ** pts_to s #(half_perm full_perm) 2
+{
+  ()
+}
+```
+
+```pulse
+fn test_share5 (r : ref int) (s : ref int)
+  requires
+        pts_to r 1
+     ** pts_to s #(half_perm full_perm) 2
+     ** pts_to s #(half_perm full_perm) 2
+  ensures  pts_to r #(half_perm full_perm) 1
+        ** pts_to r #(half_perm full_perm) 1
+        ** pts_to s #(half_perm full_perm) 2
+        ** pts_to s #(half_perm full_perm) 2
+{
+  ()
+}
+```
+
+```pulse
+fn test_gather5 (r : ref int) (s : ref int)
+  requires pts_to r #(half_perm full_perm) 1
+        ** pts_to r #(half_perm full_perm) 1
+        ** pts_to s #(half_perm full_perm) 2
+        ** pts_to s #(half_perm full_perm) 2
+  ensures 
+        pts_to r 1
+     ** pts_to s #(half_perm full_perm) 2
+     ** pts_to s #(half_perm full_perm) 2
+{
+  ()
+}
+```
+
+```pulse
+fn test_gather6 (r : ref int) (s : ref int)
+  requires pts_to s #full_perm 2
+  ensures pts_to s #(half_perm full_perm) 2
+       ** pts_to s #(half_perm (half_perm full_perm)) 2
+       ** pts_to s #(half_perm (half_perm full_perm)) 2
+{
+  ()
+}
+```
+
+```pulse
+fn test_share6 (r : ref int) (s : ref int)
+  requires pts_to s #(half_perm full_perm) 2
+       ** pts_to s #(half_perm (half_perm full_perm)) 2
+       ** pts_to s #(half_perm (half_perm full_perm)) 2
+  ensures pts_to s #full_perm 2
+{
+  gather s;
+  gather s;
+}
+```
+
