share/pulse/examples/AutoShareGather.fst
@@ -1,0 +1,237 @@
+module AutoShareGather
+
+open Pulse.Lib.Pervasives
+
+(*
+
+#set-options "--print_implicits --debug prover.share_gather"
+
+```pulse
+fn test_gather1 (r : ref int) (f:perm)
+  requires pts_to r #(f /. 2.0R) 1
+        ** pts_to r #(f /. 2.0R) 1
+  ensures pts_to r #f 1
+{
+  ();
+}
+```
+
+```pulse
+fn test_gather1_exists (r : ref int) (f:perm)
+  requires (exists* v. pts_to r #(f /. 2.0R) v)
+        ** pts_to r #(f /. 2.0R) 1
+  ensures pts_to r #f 1
+{
+  // gather r;
+  ()
+}
+```
+
+```pulse
+fn test_gather2_exists (r : ref int) (f:perm)
+  requires pts_to r #(f /. 2.0R) 1
+        ** (exists* v. pts_to r #(f /. 2.0R) v)
+  ensures pts_to r #f 1
+{
+  // gather r;
+  ()
+}
+```
+
+```pulse
+fn test_gather3_exists (r : ref int) (f:perm)
+  requires (exists* v. pts_to r #(f /. 2.0R) v)
+        ** (exists* v. pts_to r #(f /. 2.0R) v)
+  ensures (exists* v. pts_to r #f v)
+{
+  // gather r;
+  ()
+}
+```
+
+```pulse
+fn test_gather_het1 (r : ref int) (v:int) (f:perm)
+  requires pts_to r #(f /. 2.0R) 1
+        ** pts_to r #(f /. 2.0R) v
+  ensures pts_to r #f 1
+{
+  ()
+  // gather r;
+}
+```
+
+```pulse
+fn test_gather_het2 (r : ref int) (v:int) (f:perm)
+  requires pts_to r #(f /. 2.0R) 1
+        ** pts_to r #(f /. 2.0R) v
+  ensures pts_to r #f v
+{
+  // gather r;
+  ()
+}
+```
+
+```pulse
+fn test_share1 (r : ref int) (f:perm)
+  requires pts_to r #f 1
+  ensures pts_to r #(f /. 2.0R) 1
+        ** pts_to r #(f /. 2.0R) 1
+{
+  admit()
+}
+```
+
+```pulse
+fn test_gather2 (r : ref int)
+  requires pts_to r #(1.0R /. 2.0R) 1
+        ** pts_to r #((1.0R /. 2.0R) /. 2.0R) 1
+        ** pts_to r #((1.0R /. 2.0R) /. 2.0R) 1
+  ensures pts_to r 1
+{
+  assert (pts_to r #(1.0R /. 2.0R) 1 ** pts_to r #(1.0R /. 2.0R) 1);
+  ()
+}
+```
+
+```pulse
+fn test_share2 (r : ref int)
+  requires pts_to r 1
+  ensures  pts_to r #(half_perm 1.0R) 1
+        ** pts_to r #(half_perm (half_perm 1.0R)) 1
+        ** pts_to r #(half_perm (half_perm 1.0R)) 1
+{
+  ()
+}
+```
+
+```pulse
+fn test_share2_0 (r : ref int)
+  requires pts_to r 1
+  ensures  pts_to r #(half_perm (half_perm 1.0R)) 1
+        ** pts_to r #(half_perm (half_perm 1.0R)) 1
+        ** pts_to r #(half_perm (half_perm 1.0R)) 1
+        ** pts_to r #(half_perm (half_perm 1.0R)) 1
+{
+  ()
+}
+```
+
+```pulse
+fn need_quarter (r : ref int) (f:perm)
+  requires pts_to r #(half_perm (f /. 2.0R)) 1
+  ensures  pts_to r #(half_perm (f /. 2.0R)) 1
+{
+  ()
+}
+```
+
+```pulse
+fn test_call_quarter (r: ref int)
+  requires pts_to r 1
+  ensures  pts_to r 1
+{
+  need_quarter r 1.0R;
+  gather r;
+  gather r;
+}
+```
+
+
+```pulse
+fn test_gather3 (r : ref int) (s : ref int)
+  requires pts_to r #(half_perm 1.0R) 1
+        ** pts_to r #(half_perm 1.0R) 1
+        ** pts_to s 2
+  ensures pts_to r 1 ** pts_to s 2
+{
+  ()
+}
+```
+
+```pulse
+fn test_share3 (r : ref int) (s : ref int)
+  requires pts_to r 1 ** pts_to s 2
+  ensures  pts_to r #(half_perm 1.0R) 1
+        ** pts_to r #(half_perm 1.0R) 1
+        ** pts_to s 2
+{
+  ()
+}
+```
+
+```pulse
+fn test_gather4 (r : ref int) (s : ref int)
+  requires pts_to r #(half_perm 1.0R) 1
+        ** pts_to r #(half_perm 1.0R) 1
+        ** pts_to s #(half_perm 1.0R) 2
+        ** pts_to s #(half_perm 1.0R) 2
+  ensures pts_to r 1 ** pts_to s 2
+{
+  ()
+}
+```
+
+```pulse
+fn test_share4 (r : ref int) (s : ref int)
+  requires pts_to r 1 ** pts_to s 2
+  ensures  pts_to r #(half_perm 1.0R) 1
+        ** pts_to r #(half_perm 1.0R) 1
+        ** pts_to s #(half_perm 1.0R) 2
+        ** pts_to s #(half_perm 1.0R) 2
+{
+  ()
+}
+```
+
+```pulse
+fn test_share5 (r : ref int) (s : ref int)
+  requires
+        pts_to r 1
+     ** pts_to s #(half_perm 1.0R) 2
+     ** pts_to s #(half_perm 1.0R) 2
+  ensures  pts_to r #(half_perm 1.0R) 1
+        ** pts_to r #(half_perm 1.0R) 1
+        ** pts_to s #(half_perm 1.0R) 2
+        ** pts_to s #(half_perm 1.0R) 2
+{
+  ()
+}
+```
+
+```pulse
+fn test_gather5 (r : ref int) (s : ref int)
+  requires pts_to r #(half_perm 1.0R) 1
+        ** pts_to r #(half_perm 1.0R) 1
+        ** pts_to s #(half_perm 1.0R) 2
+        ** pts_to s #(half_perm 1.0R) 2
+  ensures 
+        pts_to r 1
+     ** pts_to s #(half_perm 1.0R) 2
+     ** pts_to s #(half_perm 1.0R) 2
+{
+  ()
+}
+```
+
+```pulse
+fn test_gather6 (r : ref int) (s : ref int)
+  requires pts_to s #1.0R 2
+  ensures pts_to s #(half_perm 1.0R) 2
+       ** pts_to s #(half_perm (half_perm 1.0R)) 2
+       ** pts_to s #(half_perm (half_perm 1.0R)) 2
+{
+  ()
+}
+```
+
+```pulse
+fn test_share6 (r : ref int) (s : ref int)
+  requires pts_to s #(half_perm 1.0R) 2
+       ** pts_to s #(half_perm (half_perm 1.0R)) 2
+       ** pts_to s #(half_perm (half_perm 1.0R)) 2
+  ensures pts_to s #1.0R 2
+{
+  gather s;
+  gather s;
+}
+```
