src/checker/Pulse.Checker.Prover.AutoLem.fst
@@ -1,0 +1,398 @@
+(*
+   Copyright 2023 Microsoft Research
+
+   Licensed under the Apache License, Version 2.0 (the "License");
+   you may not use this file except in compliance with the License.
+   You may obtain a copy of the License at
+
+       http://www.apache.org/licenses/LICENSE-2.0
+
+   Unless required by applicable law or agreed to in writing, software
+   distributed under the License is distributed on an "AS IS" BASIS,
+   WITHOUT WARRANTIES OR CONDITIONS OF ANY KIND, either express or implied.
+   See the License for the specific language governing permissions and
+   limitations under the License.
+*)
+
+module Pulse.Checker.Prover.AutoLem
+
+open FStar.Tactics.V2
+open FStar.Reflection.V2.TermEq
+open Pulse.Checker.Base
+open Pulse.Syntax
+open Pulse.Typing
+open Pulse.Typing.Env
+
+open Pulse.PP
+open Pulse.Show
+
+open FStar.List.Tot.Base
+
+module PS = Pulse.Checker.Prover.Substs
+module R = FStar.Reflection.V2
+module Comb = Pulse.Typing.Combinators
+module RU = Pulse.Reflection.Util
+
+let debug (g:env) (f : unit -> Tac unit) =
+  if true || Pulse.RuntimeUtils.debug_at_level (fstar_env g) "prover.autolem"
+  then f ()
+
+class tacmonad (t : Type u#a -> Type u#a) = {
+  return : #a:Type -> a -> Tac (t a);
+  ( let! ) : #a:Type -> #b:Type -> t a -> (a -> Tac (t b)) -> Tac (t b);
+}
+
+instance _ : tacmonad option = {
+  return = (fun x -> Some x);
+  ( let! ) = (fun #a #b (x : option a) (f : a -> Tac (option b)) ->
+    match x with
+    | None -> None
+    | Some x -> f x);
+}
+
+class tac_alternative (t : Type u#a) = {
+  empty : t;
+  ( <|> ) : t -> (unit -> Tac t) -> Tac t;
+}
+
+instance alternative_option (a:Type) : tac_alternative (option a) = {
+  empty = None;
+  ( <|> ) = (fun x y -> match x with None -> y () | Some _ -> x)
+}
+
+let hua (t:R.term) : Tac (option (R.fv & list universe & list argv)) =
+  let hd, args = collect_app_ln t in
+  match inspect hd with
+  | Tv_FVar fv     -> Some (fv, [], args)
+  | Tv_UInst fv us -> Some (fv, us, args)
+  | _ -> None 
+
+let eager_autolem1 (#preamble:preamble) (pst:prover_state preamble)
+  : Tac (option (pst':prover_state preamble { pst' `pst_extends` pst /\
+                                        pst'.unsolved == pst.unsolved }))
+  = 
+  None
+  // let rng = match pst.remaining_ctxt with
+  //   | [] -> FStar.Range.range_0
+  //   | v::_ -> v.range
+  // in
+
+  // debug pst.pg (fun () ->
+  //   warn_doc pst.pg (Some rng) [
+  //     text "Trying eager gather";
+  //     text "Unsolved: " ^^ pp pst.unsolved;
+  //     text "Solved: " ^^ pp pst.solved;
+  //     text "Remaining ctx: " ^^ pp pst.remaining_ctxt;
+  //   ]);
+  // match find_two_halves pst.remaining_ctxt with
+  // | None -> None
+  // | Some ((ty, r, p, e), e', v1, v2, ctxt') ->
+  //   let v = mk_pts_to v1.range ty r p e in
+
+  //   let eq : vprop = {
+  //      t = Tm_Pure (tm_fstar (RU.mk_eq2 (pack_universe Uv_Zero) ty e e') v.range);
+  //      range = v.range
+  //   } in
+
+  //   let new_ctx = v::eq::ctxt' in
+  //   let k1 :
+  //     continuation_elaborator pst.pg (Comb.list_as_vprop pst.remaining_ctxt * preamble.frame * PS.ss_term pst.solved pst.ss)
+  //                             pst.pg (Comb.list_as_vprop new_ctx * preamble.frame * PS.ss_term pst.solved pst.ss)
+  //   = fun post (| t, c, d |) ->
+  //       admit();
+  //       (| t, c, d |)
+  //   in
+  //   let k2 :
+
+  //     continuation_elaborator preamble.g0 (preamble.ctxt * preamble.frame)
+  //                             pst.pg (Comb.list_as_vprop pst.remaining_ctxt * preamble.frame * PS.ss_term pst.solved pst.ss)
+  //   = pst.k
+  //   in
+  //   let pst' = { pst with
+  //     remaining_ctxt = new_ctx;
+  //     remaining_ctxt_frame_typing = magic();
+
+  //     k = k_elab_trans k2 k1;
+  //   }
+  //   in
+  //   Some pst'
+
+let rec eager_autolem #preamble pst =
+  match eager_autolem1 pst with
+  | Some pst' -> eager_autolem pst'
+  | None -> pst
+
+let guided_autolem_attr : Reflection.term = pack (Tv_FVar (pack_fv ["Pulse"; "Lib"; "Core"; "guided_autolem"]))
+
+instance pp_fv : printable Reflection.fv = {
+  pp = (fun fv -> pp (pack (Tv_FVar fv)))
+}
+instance pp_aqualv : printable aqualv = {
+  pp = (fun x -> match x with | Q_Explicit -> text "Q_Explicit" | Q_Implicit -> text "Q_Implicit" | Q_Meta t -> text "Q_Meta" ^/^ pp t)
+}
+
+instance pp_binder : printable Tactics.NamedView.binder = {
+  pp = (fun (b:Tactics.NamedView.binder) -> pp (unseal b.ppname, b.sort, b.qual));
+}
+
+instance pp_tot_or_ghost : printable tot_or_ghost = {
+  pp = (fun x -> match x with | E_Total -> text "E_Total" | E_Ghost -> text "E_Ghost")
+}
+
+exception Retry
+
+let rec apply_first #a #b (f : a -> Tac (option b)) (cands : list a) : Tac (option b) =
+  match cands with
+  | [] -> None
+  | x::xs ->
+    match try f x with | Retry -> None | e -> raise e with
+    | Some y -> Some y
+    | None -> apply_first f xs
+    
+let n_args (typ:R.term) : Tac nat =
+  let bs, c = collect_arr typ in
+  List.length bs
+
+ 
+instance pp_comp_view : printable comp_view = {
+  pp = (fun x -> match x with
+     | C_Total ret -> text "C_Total" ^/^ pp ret
+     | C_GTotal ret -> text "C_GTotal" ^/^ pp ret
+     | C_Lemma pre post pats -> text "C_Lemma" ^/^ pp pre ^/^ pp post ^/^ pp pats
+     | C_Eff us eff_name result eff_args decrs -> text "C_Eff" ^/^ pp us ^/^ pp eff_name ^/^ pp result ^/^ pp eff_args ^/^ pp decrs
+)                 
+}
+
+(* FIXME: duplicated *)
+let binder_to_r_namedv (b:Tactics.NamedView.binder) : R.namedv =
+  R.pack_namedv {
+    uniq = b.uniq;
+    sort = seal b.sort;
+    ppname = b.ppname;
+  }
+
+let apply_wild (e:R.env) (t : R.term) (bs : binders) : Tac (R.term & subst_t & list R.term) = 
+  let rec go (t : R.term) (bs : binders) (subst : subst_t) (uvs:list R.term) : Tac (R.term & subst_t & list R.term) =
+    match bs with
+    | [] -> t, subst, uvs
+    | b::bs -> 
+      let ut = uvar_env e (Some (R.subst_term subst b.sort)) in
+      let subst' = (R.NT (binder_to_r_namedv b) ut)::subst in
+      go (Tv_App t (ut, b.qual)) bs subst' (ut::uvs)
+  in
+  go t bs [] []
+
+open FStar.Tactics.V2.SyntaxCoercions
+
+let push_binding e (b:R.binding) : Tac R.env =
+  // print ("PUSHING BINDING " ^ unseal b.ppname ^ "--" ^ show (b.uniq <: int));
+  R.push_binding e b
+
+instance _ : tac_showable R.comp = {
+  show = (fun c -> Tactics.comp_to_string c);
+}
+
+instance _ : tac_showable Tactics.NamedView.comp = {
+  show = (fun c -> show (R.pack_comp c));
+}
+
+instance _ : printable R.binding = {
+  pp = (fun (b:R.binding) -> pp (unseal b.ppname) ^^ doc_of_string "--" ^^ pp (b.uniq <: int));
+}
+
+let instantiate_fun #preamble (pst : prover_state preamble) (e:R.env) (t typ : R.term) : Tac (R.env & (*uvars*)list R.term & R.term & R.typ) =
+  let bs, c = collect_arr_bs typ in
+  // warn_doc pst.pg None [
+  //   text "Destructed" ^/^ pp typ;
+  //   text "bs =" ^/^ pp bs;
+  //   text "c =" ^/^ pp c;
+  // ];
+
+  let e' = Tactics.fold_left (fun e (b:Tactics.NamedView.binder) -> push_binding e b) e bs in
+  let t', s, uvs = apply_wild e' t bs in
+  let c = R.inspect_comp <| R.subst_comp s <| R.pack_comp c in
+  match c with
+  | C_Total ty -> e', uvs, t', ty
+  | _ -> Tactics.fail "instantiate_fun: not a total comp"
+  
+  // | Tm_Emp        : term'
+  // | Tm_Pure       : p:term -> term'
+  // | Tm_Star       : l:vprop -> r:vprop -> term'
+  // | Tm_ExistsSL   : u:universe -> b:binder -> body:vprop -> term'
+  // | Tm_ForallSL   : u:universe -> b:binder -> body:vprop -> term'
+  // | Tm_VProp      : term'
+  // | Tm_Inv        : vprop -> term'
+  // | Tm_Inames     : term'  // type inames
+  // | Tm_EmpInames  : term'
+  // | Tm_AddInv     : i:term -> is:term -> term'
+  // | Tm_FStar      : host_term -> term'
+  // | Tm_Unknown    : term'
+
+let rec explode (t:term) : Tac (list (t:R.term)) =
+  match inspect_term t with
+  | Tm_Star l r -> explode l @ explode r
+  | Tm_FStar t -> [t]
+  | _ -> []
+ 
+let rec remove1 e (ctx : list vprop) (p : R.term) : Tac (list vprop) =
+  match ctx with
+  | [] -> 
+    Tactics.print ("Could not find in ctx:" ^ show p );
+    raise Retry // Tactics.fail "vprop p in pre not found in ctx"
+  | q::qs -> if unify_env e q p then qs else q::(remove1 e qs p)
+  
+let rec remove e (ctx : list vprop) (pre : list R.term) : Tac (list vprop) =
+  match pre with
+  | [] -> ctx
+  | p::ps ->
+    print ("TRYING to remove (" ^ show p ^ ") from ctx: " ^ show ctx);
+    remove e (remove1 e ctx p) ps
+
+let typ_of_fv (fv:R.fv) : Tac R.typ =
+  match lookup_typ (top_env ()) (inspect_fv fv) with
+  | None -> Tactics.fail "sigelt not found"
+  | Some se ->
+    match inspect_sigelt se with
+    | Sg_Let {lbs=[lb]} -> lb.lb_typ
+    | Sg_Val {typ} -> typ
+    | _ -> Tactics.fail "unexpected sigelt"
+
+#push-options "--z3rlimit 20"
+let guided_autolem1 (#preamble:preamble) (pst:prover_state preamble)
+  (q:vprop) (unsolved':list vprop)
+  (_:squash (pst.unsolved == q::unsolved'))
+  (prover:prover_t)
+  (fv:Reflection.fv)
+: Tac (option (pst':prover_state preamble { pst' `pst_extends` pst }))
+=
+  let q_rng = range_of_term q in
+  debug pst.pg (fun () ->
+  warn_doc pst.pg (Some q_rng) [
+    text "Trying candidate autolem" ^/^ pp fv ^/^ text "for resource:" ^/^ pp q;
+    text "Unsolved:" ^/^ pp pst.unsolved;
+    text "Solved:" ^/^ pp pst.solved;
+    text "Remaining ctx:" ^/^ pp pst.remaining_ctxt;
+    text "env =" ^/^ pp (vars_of_env (elab_env pst.pg));
+  ]);
+  
+  let e0 = pst.pg in
+
+  let tm = pack (Tv_FVar fv) in
+  let typ = typ_of_fv fv in
+  warn_doc pst.pg (Some q_rng) [
+    text "typ = " ^/^ pp typ;
+  ];
+
+  let fe0 = elab_env e0 in
+  let e', uvs, tm, typ = instantiate_fun pst fe0 tm typ in
+  
+  match readback_comp typ with | None -> None | Some cc ->
+
+  // debug pst.pg (fun () -> warn_doc pst.pg (Some q_rng) [
+  //   text "cc = " ^/^ pp (cc <: comp);
+  // ]);
+  
+  match cc with
+  | C_Tot _ ->
+    debug pst.pg (fun () -> warn_doc pst.pg (Some q_rng) [
+      text "Skipping " ^/^ pp fv ^/^ text "because it's a total term";
+    ]);
+    None
+  | C_STAtomic _ _ _
+  | C_ST _ ->
+    debug pst.pg (fun () -> warn_doc pst.pg (Some q_rng) [
+      text "Skipping " ^/^ pp fv ^/^ text "because it's a" ^/^ pp (ctag_of_comp_st cc);
+    ]);
+    None
+  | C_STGhost _ {u; res; pre; post} ->
+    // FIXME: check res is unit
+    debug pst.pg (fun () -> warn_doc pst.pg (Some q_rng) [
+      pp fv ^/^ text "is a ghost step";
+      text "u = " ^/^ pp u;
+      text "res = " ^/^ pp res;
+      text "pre = " ^/^ pp pre;
+      text "post = " ^/^ pp (map (fun (t:(t:R.term)) -> t <: R.term) <| explode post);
+    ]);
+    match explode post with
+    | [] -> None
+    | trig::rest ->
+    // debug pst.pg (fun () ->
+    warn_doc pst.pg (Some q_rng) [
+      text "Trying to unify post with the resource";
+      text "trig = " ^/^ pp trig;
+      text "q = " ^/^ pp q;
+      text "env =" ^/^ pp (vars_of_env e');
+    ];
+    print "{{";
+    let b = unify_env e' trig q in
+    print "}}";
+    debug pst.pg (fun () -> warn_doc pst.pg (Some q_rng) [
+      text "unif result = " ^/^ pp b;
+      text "u = " ^/^ pp u;
+      text "res = " ^/^ pp res;
+      text "pre = " ^/^ pp pre;
+      text "post = " ^/^ pp (map (fun (t:(t:R.term)) -> t <: R.term) <| explode post);
+      text "t = " ^/^ pp tm;
+    ]);
+    
+    if not b then raise Retry;
+    
+    (* SUCCESS *)
+    
+    let pre' = map (fun (t:(t:R.term)) -> t <: R.term) <| explode pre in
+    let new_ctx = rest @ (remove e' pst.remaining_ctxt pre') in
+    warn_doc pst.pg (Some q_rng) [
+      text "new_ctx = " ^/^ pp new_ctx;
+    ];
+    let k1 :
+      continuation_elaborator pst.pg (list_as_vprop pst.remaining_ctxt * preamble.frame * PS.ss_term pst.solved pst.ss)
+                              pst.pg (list_as_vprop new_ctx * preamble.frame * PS.ss_term (q * pst.solved) pst.ss)
+    = fun post (| t, c, d |) ->
+        admit();
+        (| t, c, d |)
+    in
+    let k2 :
+
+      continuation_elaborator preamble.g0 (preamble.ctxt * preamble.frame)
+                              pst.pg (list_as_vprop pst.remaining_ctxt * preamble.frame * PS.ss_term pst.solved pst.ss)
+    = pst.k
+    in
+    let pst' = { pst with
+      remaining_ctxt = new_ctx;
+      remaining_ctxt_frame_typing = magic();
+
+      unsolved = unsolved';
+      solved = q * pst.solved;
+
+      goals_inv = magic();
+      solved_inv = magic();
+
+      k = k_elab_trans k2 k1;
+    }
+    in
+    Some pst'
+
+let guided_autolem (#preamble:preamble) (pst:prover_state preamble)
+  (q:vprop) (unsolved':list vprop)
+  (_:squash (pst.unsolved == q::unsolved'))
+  (prover:prover_t)
+: Tac (option (pst':prover_state preamble { pst' `pst_extends` pst }))
+=
+  let q_rng = range_of_term q in
+  debug pst.pg (fun () ->
+  warn_doc pst.pg (Some q_rng) [
+    text "Trying autolem for resource:" ^/^ pp q;
+    text "Unsolved:" ^/^ pp pst.unsolved;
+    text "Solved:" ^/^ pp pst.solved;
+    text "Remaining ctx:" ^/^ pp pst.remaining_ctxt;
+  ]);
+  
+  let cands = lookup_attr (guided_autolem_attr) (fstar_env pst.pg) in
+  
+  debug pst.pg (fun () ->
+  warn_doc pst.pg (Some q_rng) [
+    text "Candidates = " ^/^ pp cands;
+  ]);
+  
+  (* Try candidates in order, stop on first success. *)
+  cands |> apply_first (guided_autolem1 pst q unsolved' () prover)
