src/checker/Pulse.Checker.Prover.ShareGather.fst
@@ -1,0 +1,434 @@
+(*
+   Copyright 2023 Microsoft Research
+
+   Licensed under the Apache License, Version 2.0 (the "License");
+   you may not use this file except in compliance with the License.
+   You may obtain a copy of the License at
+
+       http://www.apache.org/licenses/LICENSE-2.0
+
+   Unless required by applicable law or agreed to in writing, software
+   distributed under the License is distributed on an "AS IS" BASIS,
+   WITHOUT WARRANTIES OR CONDITIONS OF ANY KIND, either express or implied.
+   See the License for the specific language governing permissions and
+   limitations under the License.
+*)
+
+module Pulse.Checker.Prover.ShareGather
+
+open FStar.Tactics.V2
+open FStar.Reflection.V2.TermEq
+open Pulse.Checker.Base
+open Pulse.Syntax
+open Pulse.Typing
+open Pulse.Typing.Env
+
+open Pulse.PP
+open Pulse.Show
+
+open FStar.List.Tot.Base
+
+module PS = Pulse.Checker.Prover.Substs
+module R = FStar.Reflection.V2
+module Comb = Pulse.Typing.Combinators
+module RU = Pulse.Reflection.Util
+
+let debug (g:env) (f : unit -> Tac unit) =
+  if Pulse.RuntimeUtils.debug_at_level (fstar_env g) "prover.share_gather"
+  then f ()
+
+class tacmonad (t : Type u#a -> Type u#a) = {
+  return : #a:Type -> a -> Tac (t a);
+  ( let! ) : #a:Type -> #b:Type -> t a -> (a -> Tac (t b)) -> Tac (t b);
+}
+
+instance _ : tacmonad option = {
+  return = (fun x -> Some x);
+  ( let! ) = (fun #a #b (x : option a) (f : a -> Tac (option b)) ->
+    match x with
+    | None -> None
+    | Some x -> f x);
+}
+
+class tac_alternative (t : Type u#a) = {
+  empty : t;
+  ( <|> ) : t -> (unit -> Tac t) -> Tac t;
+}
+
+instance alternative_option (a:Type) : tac_alternative (option a) = {
+  empty = None;
+  ( <|> ) = (fun x y -> match x with None -> y () | Some _ -> x)
+}
+
+let hua (t:R.term) : Tac (option (R.fv & list universe & list argv)) =
+  let hd, args = collect_app_ln t in
+  match inspect hd with
+  | Tv_FVar fv     -> Some (fv, [], args)
+  | Tv_UInst fv us -> Some (fv, us, args)
+  | _ -> None 
+
+let destruct_pts_to (v : vprop) : Tac (option (R.typ & R.term & R.term & R.term)) =
+  match hua v with
+  | Some (fv, _, [(ty, Q_Implicit); (r, Q_Explicit); (p, Q_Implicit); (e, Q_Explicit)]) ->
+    if inspect_fv fv = ["Pulse"; "Lib"; "Reference"; "pts_to"]
+    then Some (ty, r, p, e)
+    else None
+  | _ -> None
+
+
+(* Returns Some p' when p is of the form (p' /. 2.0R) *)
+let is_half (p:R.term) : T.Tac (option R.term) =
+  match hua p with
+  | Some (fv, [], [(perm, Q_Explicit); (denom, Q_Explicit)]) ->
+    if inspect_fv fv = ["FStar"; "Real"; "op_Slash_Dot"]
+       && term_eq denom (`2.0R)
+    then Some perm
+    else None
+  | _ -> None
+
+
+let rec destruct_halves (t : R.term) : Tac (nat & R.term) =
+  match is_half t with
+  | Some p ->
+    let n, p = destruct_halves p in
+    (n + 1, p)
+  | _ -> (0, t)
+
+let destruct_pts_to_half_n (v : vprop) : Tac (option (nat & R.typ & R.term & R.term & R.term)) =
+  match destruct_pts_to v with
+  | Some (ty, r, p, e) -> (
+    let n, p = destruct_halves p in
+    Some (n, ty, r, p, e)
+  )
+  | _ -> None
+
+let destruct_pts_to_half (v : vprop) : Tac (option (R.typ & R.term & R.term & R.term)) =
+  match destruct_pts_to v with
+  | Some (ty, r, p, e) -> (
+    (match is_half p with
+     | Some p' -> Some (ty, r, p', e)
+     | None -> None)
+  )
+  | _ -> None
+
+let is_pts_to (t_r t_p t_e : R.term) (v : vprop) : Tac bool =
+  match destruct_pts_to v with
+  | Some (_, r, p, e) -> term_eq t_r r && term_eq t_p p && term_eq t_e e
+  | None -> false
+
+let is_pts_to_half_any (t_r t_p : R.term) (v : vprop) : Tac (option R.term) =
+  match destruct_pts_to_half v with
+  | Some (_, r, p, e) ->
+    if term_eq t_r r && term_eq t_p p
+    then Some e
+    else None
+  | None -> None
+
+let is_pts_to_half (t_r t_p t_e : R.term) (v : vprop) : Tac bool =
+  match destruct_pts_to_half v with
+  | Some (_, r, p, e) -> term_eq t_r r && term_eq t_p p && term_eq t_e e
+  | None -> false
+  
+let mk_pts_to rng (ty r p e : R.term) : term =
+  mk_app (pack (Tv_FVar (pack_fv ["Pulse"; "Lib"; "Reference"; "pts_to"]))) [
+    (ty, Q_Implicit);
+    (r, Q_Explicit);
+    (p, Q_Implicit);
+    (e, Q_Explicit);
+  ]
+
+let rec find_pts_to (t_r t_p t_v : R.term) (ctx : list vprop) : Tac (option (vprop & list vprop)) =
+  match ctx with
+  | [] -> None
+  | v::vs ->
+    if is_pts_to t_r t_p t_v v then
+      Some (v, vs)
+    else
+      let! (v', vs) = find_pts_to t_r t_p t_v vs in
+      return (v', v::vs)
+
+let rec find_pts_to_half (t_r t_p t_v : R.term) (ctx : list vprop) : Tac (option (vprop & list vprop)) =
+  match ctx with
+  | [] -> None
+  | v::vs ->
+    if is_pts_to_half t_r t_p t_v v then
+      Some (v, vs)
+    else
+      let! (v', vs) = find_pts_to_half t_r t_p t_v vs in
+      return (v', v::vs)
+
+let rec find_pts_to_half_any (t_r t_p : R.term) (ctx : list vprop) : Tac (option (R.term & vprop & list vprop)) =
+  match ctx with
+  | [] -> None
+  | v::vs ->
+    match is_pts_to_half_any t_r t_p v with
+    | Some e -> Some (e, v, vs)
+    | None ->
+      let! (e', v', vs) = find_pts_to_half_any t_r t_p vs in
+      return (e', v', v::vs)
+
+let rec find_two_halves (ctx : list vprop) : Tac (option ((R.typ & R.term & R.term & R.term) & R.term & vprop & vprop & list vprop)) =
+  match ctx with
+  | [] -> None
+  | v::vs ->
+    let fallback () =
+      let! (r, e, v1, v2, vs) = find_two_halves vs in
+      Some (r, e, v1, v2, v::vs)
+    in
+    (
+      let! (ty, r, p, e) = destruct_pts_to_half v in
+      let! (e', v', vs') = find_pts_to_half_any r p vs in
+      Some ((ty, r, p, e), e', v, v', vs')
+     ) <|> fallback
+
+let eager_gather1 (#preamble:preamble) (pst:prover_state preamble)
+  : T.Tac (option (pst':prover_state preamble { pst' `pst_extends` pst /\
+                                        pst'.unsolved == pst.unsolved }))
+  = 
+  let rng = match pst.remaining_ctxt with
+    | [] -> FStar.Range.range_0
+    | v::_ -> range_of_term v
+  in
+
+  debug pst.pg (fun () ->
+    warn_doc pst.pg (Some rng) [
+      text "Trying eager gather";
+      text "Unsolved: " ^^ pp pst.unsolved;
+      text "Solved: " ^^ pp pst.solved;
+      text "Remaining ctx: " ^^ pp pst.remaining_ctxt;
+    ]);
+  match find_two_halves pst.remaining_ctxt with
+  | None ->
+    T.print "No two halves found";
+    None
+  | Some ((ty, r, p, e), e', v1, v2, ctxt') ->
+    let v = mk_pts_to (range_of_term v1) ty r p e in
+
+    let eq : vprop = tm_pure (RU.mk_eq2 (pack_universe Uv_Zero) ty e e') in
+
+    let new_ctx = v::eq::ctxt' in
+    let k1 :
+      continuation_elaborator pst.pg (list_as_vprop pst.remaining_ctxt * preamble.frame * PS.ss_term pst.solved pst.ss)
+                              pst.pg (list_as_vprop new_ctx * preamble.frame * PS.ss_term pst.solved pst.ss)
+    = fun post (| t, c, d |) ->
+        admit();
+        (| t, c, d |)
+    in
+    let k2 :
+
+      continuation_elaborator preamble.g0 (preamble.ctxt * preamble.frame)
+                              pst.pg (list_as_vprop pst.remaining_ctxt * preamble.frame * PS.ss_term pst.solved pst.ss)
+    = pst.k
+    in
+    let pst' = { pst with
+      remaining_ctxt = new_ctx;
+      remaining_ctxt_frame_typing = magic();
+
+      k = k_elab_trans k2 k1;
+    }
+    in
+    Some pst'
+
+let rec eager_gather #preamble pst =
+  match eager_gather1 pst with
+  | Some pst' -> eager_gather { pst' with progress = true }
+  | None -> pst
+  
+let rec mk_n_half (n:nat) (p : R.term) : R.term =
+  if n = 0
+  then p
+  else
+  mk_e_app
+    (pack (Tv_FVar (pack_fv ["FStar"; "Real"; "op_Slash_Dot"])))
+    [
+      (mk_n_half (n - 1) p);
+      (`2.0R);	
+    ]
+  
+let mk_half (p : R.term) : R.term = mk_n_half 1 p
+
+let rec find_least_split (nsplits : nat) (ty r p e : R.term) (ctx : list vprop)
+: Tac (option (
+      (* number of splits *) nat &
+      (* perm  *) R.term &
+      (* the matched vprop *) vprop &
+      (* other halves breakdown *) list vprop &
+      (* rest of ctx *)list vprop))
+=
+  let p' = mk_n_half nsplits p in
+  match find_pts_to r p' e ctx with
+  | None ->
+    if nsplits > 0
+    then 
+      let other_half = mk_pts_to Range.range_0 ty r p' e in
+      let! (n, p', v, hs, ctx') = find_least_split (nsplits - 1) ty r p e ctx in
+      Some (n, p', v, other_half::hs, ctx')
+    else None
+  | Some (v, ctxt') ->
+    Some (nsplits, p', v, [], ctxt')
+
+let share (#preamble:preamble) (pst:prover_state preamble)
+  (q:vprop) (unsolved':list vprop)
+  (_:squash (pst.unsolved == q::unsolved'))
+  (prover:prover_t)
+: T.Tac (option (pst':prover_state preamble { pst' `pst_extends` pst }))
+=
+  let q_rng = range_of_term q in
+  debug pst.pg (fun () ->
+  warn_doc pst.pg (Some q_rng) [
+    text "Trying share for resource:" ^/^ pp q;
+    text "Unsolved:" ^/^ pp pst.unsolved;
+    text "Solved:" ^/^ pp pst.solved;
+    text "Remaining ctx:" ^/^ pp pst.remaining_ctxt;
+  ]);
+
+  match destruct_pts_to_half_n q with
+  | None ->
+    debug pst.pg (fun () ->
+    warn_doc pst.pg (Some (range_of_term q)) [
+      text "Goal is not a pts_to";
+    ]);
+    None
+  | Some (nsplits, ty, r, p, e) ->
+  (* We got pts_to r #(full / 2^nsplits) e *)
+
+  (* Find some pts_to r #(full / 2^n) e in the context, with n <= nsplits *)
+  match find_least_split nsplits ty r p e pst.remaining_ctxt with
+  | None ->
+    debug pst.pg (fun () ->
+    warn_doc pst.pg (Some q_rng) [
+      text "NO SPLIT FOUND"
+    ]);
+    None
+  | Some (n', p', v, hs, ctxt') ->
+  
+  debug pst.pg (fun () ->
+  warn_doc pst.pg (Some q_rng) [
+    text "Found half of: " ^/^ pp q ^/^ text "in ctx" ^/^ pp ((n' <: int), p', v, hs, ctxt');
+  ]);
+  
+  let new_ctx = hs@ctxt' in
+  let k1 :
+    continuation_elaborator pst.pg (list_as_vprop pst.remaining_ctxt * preamble.frame * PS.ss_term pst.solved pst.ss)
+                            pst.pg (list_as_vprop new_ctx * preamble.frame * PS.ss_term (q * pst.solved) pst.ss)
+  = fun post (| t, c, d |) ->
+      admit();
+      (| t, c, d |)
+  in
+  let k2 :
+
+    continuation_elaborator preamble.g0 (preamble.ctxt * preamble.frame)
+                            pst.pg (list_as_vprop pst.remaining_ctxt * preamble.frame * PS.ss_term pst.solved pst.ss)
+  = pst.k
+  in
+  let pst' = { pst with
+    remaining_ctxt = new_ctx;
+    remaining_ctxt_frame_typing = magic();
+    
+    unsolved = unsolved';
+    solved = q * pst.solved;
+
+    goals_inv = magic();
+    solved_inv = magic();
+
+    k = k_elab_trans k2 k1;
+  }
+  in
+  Some pst'
+
+let gather (#preamble:preamble) (pst:prover_state preamble)
+  (q:vprop) (unsolved':list vprop)
+  (_:squash (pst.unsolved == q::unsolved'))
+  (prover:prover_t)
+: T.Tac (option (pst':prover_state preamble { pst' `pst_extends` pst }))
+=
+  let q_rng = range_of_term q in
+  debug pst.pg (fun () ->
+  warn_doc pst.pg (Some q_rng) [
+    text "Trying gather for resource:" ^/^ pp q;
+    text "Unsolved:" ^/^ pp pst.unsolved;
+    text "Solved:" ^/^ pp pst.solved;
+    text "Remaining ctx:" ^/^ pp pst.remaining_ctxt;
+  ]);
+
+  match destruct_pts_to q with
+  | None ->
+    debug pst.pg (fun () ->
+    warn_doc pst.pg (Some q_rng) [
+      text "Goal is not a pts_to";
+    ]);
+    None
+  | Some (ty, r, p, e) ->
+  (* We got pts_to #ty r #p e *)
+
+  (* Is the same vprop already in the context? *)
+  match find_pts_to r p e pst.remaining_ctxt with
+  | Some (v, ctxt') -> (
+    let new_ctx = ctxt' in
+    let k1 :
+      continuation_elaborator pst.pg (list_as_vprop pst.remaining_ctxt * preamble.frame * PS.ss_term pst.solved pst.ss)
+                              pst.pg (list_as_vprop new_ctx * preamble.frame * PS.ss_term (q * pst.solved) pst.ss)
+    = fun post (| t, c, d |) ->
+        admit();
+        (| t, c, d |)
+    in
+    let k2 :
+
+      continuation_elaborator preamble.g0 (preamble.ctxt * preamble.frame)
+                              pst.pg (list_as_vprop pst.remaining_ctxt * preamble.frame * PS.ss_term pst.solved pst.ss)
+    = pst.k
+    in
+    let pst' = { pst with
+      remaining_ctxt = new_ctx;
+      remaining_ctxt_frame_typing = magic();
+
+      unsolved = unsolved';
+      solved = q * pst.solved;
+
+      goals_inv = magic();
+      solved_inv = magic();
+
+      k = k_elab_trans k2 k1;
+    }
+    in
+    Some pst'
+  )
+
+  | None ->
+    (* Not exactly in ctxt, is are there two pts_to #ty r #(p /. 2.0R) e? *)
+    match find_pts_to_half r p e pst.remaining_ctxt with
+    | None ->
+      None
+    | Some (v, ctxt') ->
+      match find_pts_to_half r p e ctxt' with
+      | None ->
+        None
+      | Some (v', ctxt'') ->
+        let new_ctx = ctxt'' in
+        let k1 :
+          continuation_elaborator pst.pg (list_as_vprop pst.remaining_ctxt * preamble.frame * PS.ss_term pst.solved pst.ss)
+                                  pst.pg (list_as_vprop new_ctx * preamble.frame * PS.ss_term (q * pst.solved) pst.ss)
+        = fun post (| t, c, d |) ->
+            admit();
+            (| t, c, d |)
+        in
+        let k2 :
+
+          continuation_elaborator preamble.g0 (preamble.ctxt * preamble.frame)
+                                  pst.pg (list_as_vprop pst.remaining_ctxt * preamble.frame * PS.ss_term pst.solved pst.ss)
+        = pst.k
+        in
+        let pst' = { pst with
+          remaining_ctxt = new_ctx;
+          remaining_ctxt_frame_typing = magic();
+
+          unsolved = unsolved';
+          solved = q * pst.solved;
+
+          goals_inv = magic();
+          solved_inv = magic();
+
+          k = k_elab_trans k2 k1;
+        }
+        in
+        Some pst'
